mv

Foundation/Modal/Kripke/Basic.lean
@@ -40,89 +40,8 @@ infix:45 " ≺ " => Frame.Rel'
 abbrev RelItr' (n : ℕ) := F.Rel.iterate n
 notation x:45 " ≺^[" n "] " y:46 => Frame.RelItr' n x y
 
-abbrev RelReflTransGen : _root_.Rel F.World F.World := ReflTransGen (· ≺ ·)
-infix:45 " ≺^* " => Frame.RelReflTransGen
-
-namespace RelReflTransGen
-
-lemma single (hxy : x ≺ y) : x ≺^* y := ReflTransGen.single hxy
-
-@[simp]
-protected lemma reflexive : Reflexive F.RelReflTransGen := Relation.reflexive_reflTransGen
-
-@[simp]
-lemma refl {x : F.World} : x ≺^* x := RelReflTransGen.reflexive x
-
-@[simp]
-protected lemma transitive : Transitive F.RelReflTransGen := Relation.transitive_reflTransGen
-
-protected lemma symmetric : Symmetric F.Rel → Symmetric F.RelReflTransGen := ReflTransGen.symmetric
-
-protected lemma exists_itr : x ≺^* y ↔ ∃ n, F.Rel.iterate n x y := ReflTransGen.exists_iterate
-
-end RelReflTransGen
-
-abbrev TransitiveReflexiveClosure (F : Frame) : Frame := ⟨F.World, (· ≺^* ·)⟩
-postfix:95 "^*" => Frame.TransitiveReflexiveClosure
-
-
-abbrev RelTransGen {F : Frame} : _root_.Rel F.World F.World := TransGen (· ≺ ·)
-infix:45 " ≺^+ " => Frame.RelTransGen
-
-namespace RelTransGen
-
-protected lemma single (hxy : x ≺ y) : x ≺^+ y := TransGen.single hxy
-
-@[simp]
-protected lemma transitive : Transitive F.RelTransGen := λ _ _ _ => TransGen.trans
-
-protected lemma symmetric (hSymm : Symmetric F.Rel) : Symmetric F.RelTransGen := by
-  intro x y rxy;
-  induction rxy with
-  | single h => exact TransGen.single $ hSymm h;
-  | tail _ hyz ih => exact TransGen.trans (TransGen.single $ hSymm hyz) ih
-
-lemma exists_itr : x ≺^+ y ↔ ∃ n > 0, F.Rel.iterate n x y := TransGen.exists_iterate
-
-end RelTransGen
-
-abbrev TransitiveClosure (F : Frame) : Frame := ⟨F.World, (· ≺^+ ·)⟩
-postfix:95 "^+" => Frame.TransitiveClosure
-
-
-abbrev RelReflGen : _root_.Rel F.World F.World := ReflGen (· ≺ ·)
-infix:45 " ≺^= " => Frame.RelReflGen
-
-def ReflexiveClosure (F : Frame) : Frame := ⟨F.World, (· ≺^= ·)⟩
-postfix:95 "^=" => Frame.ReflexiveClosure
-
-
-abbrev RelIrreflGen : _root_.Rel F.World F.World := IrreflGen (· ≺ ·)
-scoped infix:45 " ≺^≠ " => Frame.RelIrreflGen
-
-def IrreflexiveClosure (F : Frame) : Frame := ⟨F.World, (· ≺^≠ ·)⟩
-postfix:95 "^≠" => Frame.IrreflexiveClosure
-
-namespace IrreflexiveClosure
-
-@[simp]
-lemma rel_irreflexive : Irreflexive (F^≠.Rel) := by
-  simp [Irreflexive, Frame.RelIrreflGen, IrreflGen, Frame.IrreflexiveClosure]
-
-end IrreflexiveClosure
-
 end Frame
 
-
-instance {F : FiniteFrame} : Finite (F.toFrame^=).World := by simp [Frame.ReflexiveClosure];
-
-abbrev FiniteFrame.ReflexiveClosure (F : FiniteFrame) : FiniteFrame := ⟨F.toFrame^=⟩
-postfix:95 "^=" => FiniteFrame.ReflexiveClosure
-
-instance {F : FiniteFrame} : Finite (F.toFrame^≠).World := by simp [Frame.IrreflexiveClosure]
-
-abbrev FiniteFrame.IrreflexiveClosure (F : FiniteFrame) : FiniteFrame := ⟨F.toFrame^≠⟩
-postfix:95 "^≠" => FiniteFrame.IrreflexiveClosure
 
 
 section
